src/hls/RTLPar.v
@@ -52,16 +52,19 @@ Section RELSEM.
 
   Inductive step: state -> trace -> state -> Prop :=
   | exec_bblock:
-    forall s (f: function) sp pc rs rs' m m' t s' bb pr pr',
-      f.(fn_code)!pc = Some bb ->
-      step_instr_block sp (mk_instr_state rs pr m) bb.(bb_body)
+    forall s f sp pc rs rs' m m' bb pr pr',
+      step_instr_block sp (mk_instr_state rs pr m) bb
                           (mk_instr_state rs' pr' m') ->
-      step_cf_instr ge (State s f sp pc (mk_bblock nil bb.(bb_exit)) rs' pr' m') t s' ->
-      step (State s f sp pc bb rs pr m) t s'
+      step (State s f sp pc bb rs pr m) E0 (JumpState s f sp pc rs' pr' m')
+  | exec_jumpstate :
+    forall s f sp pc rs pr m block t st,
+      f.(fn_code) ! pc = Some block ->
+      step_cf_instr ge (JumpState s f sp pc rs pr m) block.(bb_exit) t st ->
+      step (JumpState s f sp pc rs pr m) t st
   | exec_function_internal:
-    forall s f args m m' stk bb,
+    forall s f args m m' stk bb cf,
       Mem.alloc m 0 f.(fn_stacksize) = (m', stk) ->
-      f.(fn_code) ! (f.(fn_entrypoint)) = Some bb ->
+      f.(fn_code) ! (f.(fn_entrypoint)) = Some (mk_bblock bb cf) ->
       step (Callstate s (Internal f) args m)
         E0 (State s
                   f
@@ -75,11 +78,11 @@ Section RELSEM.
     forall s ef args res t m m',
       external_call ef ge args m t res m' ->
       step (Callstate s (External ef) args m)
-         t (Returnstate s res m')
+           t (Returnstate s res m')
   | exec_return:
-    forall res f sp pc rs s vres m pr bb,
-      step (Returnstate (Stackframe res f sp pc bb rs pr :: s) vres m)
-        E0 (State s f sp pc bb (rs#res <- vres) pr m).
+    forall res f sp pc rs s vres m pr,
+      step (Returnstate (Stackframe res f sp pc rs pr :: s) vres m)
+        E0 (State s f sp pc nil (rs#res <- vres) pr m).
 
 End RELSEM.
 
